Core/Node.v
@@ -223,8 +223,8 @@ Definition procMsg (st: State) (from : NodeId) (msg: Message) (ts: Timestamp) :=
     let: Node n prs bt pool := st in
     match msg with
     | BlockMsg b =>
-      let: newBt := btExtend bt b in
-      let: newPool := [seq t <- pool | txValid t (btChain newBt)] in
+      let: newBt := bfExtend bt b in
+      let: newPool := [seq t <- pool | txValid t (bfChain newBt)] in
       let: ownHashes := (keys_of newBt) ++ [seq hashT t | t <- newPool] in
       pair (Node n prs newBt newPool) (emitBroadcast n prs (InvMsg ownHashes))
 
@@ -262,7 +262,7 @@ Definition procInt (st : State) (tr : InternalTransition) (ts : Timestamp) :=
 
     (* Assumption: nodes broadcast to themselves as well! => simplifies logic *)
     | MintT =>
-      let: bc := btChain bt in
+      let: bc := bfChain bt in
       let: allowedTxs := [seq t <- pool | txValid t bc] in
       match genProof n bc allowedTxs ts with
       | Some pf =>
@@ -270,8 +270,8 @@ Definition procInt (st : State) (tr : InternalTransition) (ts : Timestamp) :=
           let: prevBlock := last GenesisBlock bc in
           let: block := mkB (hashB prevBlock) allowedTxs pf in
           if tx_valid_block bc block then
-            let: newBt := btExtend bt block in
-            let: newPool := [seq t <- pool | txValid t (btChain newBt)] in
+            let: newBt := bfExtend bt block in
+            let: newPool := [seq t <- pool | txValid t (bfChain newBt)] in
             let: ownHashes := (keys_of newBt) ++ [seq hashT t | t <- newPool] in
             pair (Node n prs newBt newPool) (emitBroadcast n prs (BlockMsg block))
           else
